Move [bounded_effects] over, and document all the exposed functions.

vale/code/lib/transformers/Vale.Transformers.BoundedInstructionEffects.fsti
@@ -2,6 +2,7 @@ module Vale.Transformers.BoundedInstructionEffects
 
 open Vale.X64.Machine_Semantics_s
 
+open Vale.Transformers.PossiblyMonad
 open Vale.Transformers.Locations
 
 (** An [rw_set] is the pair of [locations] that are respectively read
@@ -11,3 +12,44 @@ type rw_set = locations & locations
 (** [rw_set_of_ins i] returns the read/write sets for the execution of
     an instruction. *)
 val rw_set_of_ins : i:ins -> rw_set
+
+(** [unchanged_except exc s1 s2] means all locations that are disjoint
+    from the exceptions [exc] have the same value in both [s1] and [s2]. *)
+let unchanged_except (exceptions:locations) (s1 s2:machine_state) :
+  GTot Type0 =
+  (forall (a:location). {:pattern (eval_location a s2)} (
+      (!!(disjoint_location_from_locations a exceptions) ==>
+       (eval_location a s1 == eval_location a s2))
+    ))
+
+(** [only_affects locs f] means that running [f] leaves everything
+    except [locs] unchanged. *)
+let only_affects (locs:locations) (f:st unit) : GTot Type0 =
+  forall s. {:pattern unchanged_except locs s (run f s)} (
+    unchanged_except locs s (run f s)
+  )
+
+(** [unchanged_at locs s1 s2] means the the value of any location in
+    [locs] is same in both [s1] and [s2]. *)
+let rec unchanged_at (locs:locations) (s1 s2:machine_state) : GTot Type0 =
+  match locs with
+  | [] -> True
+  | x :: xs -> (
+      (eval_location x s1 == eval_location x s2) /\
+      (unchanged_at xs s1 s2)
+    )
+
+(** [bounded_effects r w f] means that the execution of [f] is bounded
+    by the read-set [r] and write-set [w]. This means that whenever
+    two different states are same at the locations in [r], then the
+    function will have the same effect, and that its effect is bounded
+    to the set [w]. *)
+let bounded_effects (reads writes:locations) (f:st unit) : GTot Type0 =
+  (only_affects writes f) /\
+  (
+    forall s1 s2. {:pattern unchanged_at writes (run f s1) (run f s2)} (
+      unchanged_at reads s1 s2 ==>
+      (unchanged_at writes (run f s1) (run f s2) /\
+       (run f s1).ms_ok = (run f s2).ms_ok)
+    )
+  )
